\begin{tabular}{c|c|c|c} 
    & \begin{minipage}{.25\textwidth} \centerline{Conjunctive}
   \centerline{\rule[-10pt]{0pt}{10pt}version (合取形式)} \end{minipage} & 
   \begin{minipage}{.25\textwidth} \centerline{Disjunctive}
   \centerline{\rule[-10pt]{0pt}{10pt}version (析取形式)} \end{minipage} & 
   \begin{minipage}{.25\textwidth} \centerline{Algebraic}
   \centerline{\rule[-10pt]{0pt}{10pt}analog (代数类比)} \end{minipage} \\ \hline
   \begin{minipage}{.25\textwidth} \rule{0pt}{22pt}\index{commutative law}Commutative \\ \rule{12pt}{0pt} laws (交换律)\rule[-10pt]{0pt}{10pt} \end{minipage} & 
   \begin{minipage}{.25\textwidth} \centerline{$A \land B \cong B \land A$} \end{minipage} & 
   \begin{minipage}{.25\textwidth} \centerline{$A \lor B \cong B \lor A$} \end{minipage} & 
   \begin{minipage}{.25\textwidth} \centerline{$2+3 = 3+2$}  \end{minipage}  \\ \hline
   \begin{minipage}{.25\textwidth} \rule{0pt}{22pt}\index{associative law}Associative \\ \rule{12pt}{0pt} laws (结合律)\rule[-10pt]{0pt}{10pt} \end{minipage} & 
   \begin{minipage}{.25\textwidth} \centerline{$A \land (B \land C)$\rule{16pt}{0pt}} 
   \centerline{\rule{16pt}{0pt} $\cong (A \land B) \land C $}\end{minipage} &
   \begin{minipage}{.25\textwidth} \centerline{$A \lor (B \lor C)$ \rule{16pt}{0pt}}
   \centerline{\rule{16pt}{0pt} $\cong (A \lor B) \lor C $} \end{minipage} & 
   \begin{minipage}{.25\textwidth} 
   \centerline{$2+(3+4) $ \rule{16pt}{0pt}} 
   \centerline{\rule{24pt}{0pt} $= (2+3)+4$} \end{minipage} \\ \hline 
   \begin{minipage}{.25\textwidth} 
   \rule{0pt}{22pt}\index{distributive law}Distributive \\ \rule{12pt}{0pt} laws (分配律)\rule[-10pt]{0pt}{10pt} \end{minipage} &  
   \begin{minipage}{.25\textwidth} 
   \centerline{$A \land (B \lor C) \cong $ \rule{16pt}{0pt}} 
   \centerline{$(A \land B) \lor (A \land C)$} \end{minipage} & 
   \begin{minipage}{.25\textwidth} \centerline{$A \lor (B \land C) \cong $ \rule{16pt}{0pt}} 
   \centerline{$(A \lor B) \land (A \lor C)$} \end{minipage} & 
   \begin{minipage}{.25\textwidth} 
   \centerline{$2\cdot(3+4) $ \rule{16pt}{0pt}}
   \centerline{\rule{16pt}{0pt} $ = (2\cdot 3 + 2\cdot 4)$} \end{minipage} \\ \hline 
   \begin{minipage}{.25\textwidth} \rule{0pt}{22pt}\index{DeMorgan's law}DeMorgan's \\ \rule{12pt}{0pt} laws (德摩根定律)\rule[-10pt]{0pt}{10pt} \end{minipage} & 
   \begin{minipage}{.25\textwidth} \centerline{${\lnot}(A \land B)$ \rule{25pt}{0pt}}
   \centerline{ \rule{16pt}{0pt} $ \cong \; {\lnot}A \lor {\lnot}B$} \end{minipage} & 
   \begin{minipage}{.25\textwidth} \centerline{${\lnot}(A \lor B)$\rule{25pt}{0pt}}
   \centerline{ \rule{16pt}{0pt} $\cong \; {\lnot}A \land {\lnot}B$} \end{minipage} & none (无) \\ \hline 
   \begin{minipage}{.25\textwidth} \rule{0pt}{22pt}\index{double negation}Double negation (双重否定)\rule[-10pt]{0pt}{10pt}   \end{minipage} & 
   \begin{minipage}{.25\textwidth} \centerline{${\lnot}({\lnot}A) \; \cong \; A$}  \end{minipage} & 
   \begin{minipage}{.25\textwidth} \centerline{same (同左)} \end{minipage} & $-(-2) = 2$ \\ \hline 
   
   \begin{minipage}{.25\textwidth} \rule{0pt}{22pt}\index{complementarity law}Complementarity (互补律)\rule[-10pt]{0pt}{10pt} \end{minipage} & 
   \begin{minipage}{.25\textwidth} \centerline{$A \land {\lnot}A \; \cong \; c$} \end{minipage} & 
   \begin{minipage}{.25\textwidth} \centerline{$A \lor {\lnot}A \; \cong \; t$} \end{minipage} &  
   \begin{minipage}{.25\textwidth} \centerline{$2 + (-2) = 0$} \end{minipage} \\ \hline 
   \begin{minipage}{.25\textwidth} \rule{0pt}{22pt}\index{identity law}Identity \\ \rule{12pt}{0pt} laws (同一律)\rule[-10pt]{0pt}{10pt} \end{minipage} & 
   \begin{minipage}{.25\textwidth} \centerline{$A \land t \cong A$} \end{minipage} & 
   \begin{minipage}{.25\textwidth} \centerline{$A \lor c \cong A$} \end{minipage} & 
   \begin{minipage}{.25\textwidth} \centerline{$7 + 0 = 7$} \end{minipage}\\ \hline 
   \begin{minipage}{.25\textwidth} \rule{0pt}{22pt}\index{domination law}Domination (统治律)\rule[-10pt]{0pt}{10pt} \end{minipage} & 
   \begin{minipage}{.25\textwidth}  \centerline{$A \land c \cong c$} \end{minipage} & 
   \begin{minipage}{.25\textwidth} \centerline{$A \lor t \cong t$} \end{minipage} & 
   \begin{minipage}{.25\textwidth} \centerline{$7 \cdot 0 = 0$} \end{minipage}\\ \hline
   \begin{minipage}{.25\textwidth} \rule{0pt}{22pt}\index{idempotence}Idempotence (幂等律)\rule[-10pt]{0pt}{10pt} \end{minipage} & 
   \begin{minipage}{.25\textwidth} \centerline{$A \land A \cong A$} \end{minipage} & 
   \begin{minipage}{.25\textwidth} \centerline{$A \lor A \cong A$} \end{minipage} & 
   \begin{minipage}{.25\textwidth} \centerline{$ 1 \cdot 1 = 1$} \end{minipage} \\ \hline
   \begin{minipage}{.25\textwidth} \rule{0pt}{22pt}\index{absorption}Absorption (吸收律)\rule[-10pt]{0pt}{10pt} \end{minipage} & 
   \begin{minipage}{.25\textwidth} \centerline{$A \land (A \lor B) \cong A$} \end{minipage} & 
   \begin{minipage}{.25\textwidth} \centerline{$A \lor (A \land B) \cong A$} \end{minipage} & none (无) \\ \hline
   \begin{minipage}{.25\textwidth} \rule{0pt}{22pt}\index{equivalent forms of conditionals}Equivalent forms\\ \rule{6pt}{0pt} for conditionals (条件句的等价形式)\rule[-10pt]{0pt}{10pt} \end{minipage} & 
   \begin{minipage}{.25\textwidth} \centerline{$\lnot (A \implies B)$\rule{16pt}{0pt}} 
   \centerline{\rule{16pt}{0pt} $\cong A \land \lnot B$}\end{minipage} &
   \begin{minipage}{.25\textwidth} \centerline{$A \implies B$\rule{16pt}{0pt}} 
   \centerline{\rule{16pt}{0pt} $\cong \lnot A \lor B$}\end{minipage} & none (无) \\
   \end{tabular}